Verify Assignment forwarding pass
Had to change implementation from collect, then apply, to iteratively
applying each assignment to the ones after it. This requires the
module to be sorted, but that is easy enough to do and trivially
correct (since sorting is already part of the semantics).

Also needed to prove some properties about sorting algorithm (result
is sorted, a permutation of the input, and the sort is stable)

Commits
- WIP module_body_inline proof done - Missing collect_substitutions proof
- WIP Use substitution record everywhere
- WIP Fix definition of module_items_sorted
- WIP Reorganized AssignmentForwarding
- WIP on assignment_forwarding proof - admitted lemmas
- WIP applying a substitution does not invalidate the others
- WIP Completely change approach for assignment forwarding
- WIP Qed (with small assumption) on assignment forwarding
  Need to move sort_module_items_idempotent to VerilogSort
- SQUASHME Prove all required properties of sorting
- SQUASHME No assumptions left in assignment_forwarding

vera/AssignmentForwarding/AssignmentForwarding.v
@@ -20,76 +20,58 @@ Import MonadLetNotation.
 Local Open Scope monad_scope.
 Local Open Scope string_scope.
 
-Record substitution :=
-  MkSubstitution {
-    var : variable;
-    expr : expression (varType var)
-  }.
-
 Section inline_one.
-  Context (var : variable).
-  Context (replacement : expression (varType var)).
+  Context (var : Verilog.variable).
+  Context (replacement : Verilog.expression (Verilog.varType var)).
 
   Equations
-    expr_inline_var {w} : expression w -> expression w := {
+    apply_substitution_expr {w} : expression w -> expression w := {
     | NamedExpression other_var with (dec (other_var = var)) => {
       | left eq_refl => replacement
       | right _ => NamedExpression other_var
     }
     (* These just walk the tree *)
-    | ArithmeticOp op lhs rhs => ArithmeticOp op (expr_inline_var lhs) (expr_inline_var rhs)
-    | BitwiseOp op lhs rhs => (BitwiseOp op (expr_inline_var lhs) (expr_inline_var rhs))
-    | ShiftOp op lhs rhs => (ShiftOp op (expr_inline_var lhs) (expr_inline_var rhs))
-    | UnaryOp p e => (UnaryOp p (expr_inline_var e))
-    | Conditional cond ifT ifF => (Conditional (expr_inline_var cond) (expr_inline_var ifT) (expr_inline_var ifF))
-    | BitSelect vec idx => BitSelect (expr_inline_var vec) (expr_inline_var idx)
-    | Concatenation lhs rhs => (Concatenation (expr_inline_var lhs) (expr_inline_var rhs))
+    | ArithmeticOp op lhs rhs => ArithmeticOp op (apply_substitution_expr lhs) (apply_substitution_expr rhs)
+    | BitwiseOp op lhs rhs => (BitwiseOp op (apply_substitution_expr lhs) (apply_substitution_expr rhs))
+    | ShiftOp op lhs rhs => (ShiftOp op (apply_substitution_expr lhs) (apply_substitution_expr rhs))
+    | UnaryOp p e => (UnaryOp p (apply_substitution_expr e))
+    | Conditional cond ifT ifF => (Conditional (apply_substitution_expr cond) (apply_substitution_expr ifT) (apply_substitution_expr ifF))
+    | BitSelect vec idx => BitSelect (apply_substitution_expr vec) (apply_substitution_expr idx)
+    | Concatenation lhs rhs => (Concatenation (apply_substitution_expr lhs) (apply_substitution_expr rhs))
     | IntegerLiteral _ val => IntegerLiteral _ val
-    | Resize to e => (Resize to (expr_inline_var e))
+    | Resize to e => (Resize to (apply_substitution_expr e))
     }.
 
   Equations
-    stmt_inline_var : statement -> statement := {
-    | BlockingAssign lhs rhs => BlockingAssign lhs (expr_inline_var rhs)
-    }.
-
-  Equations
-    module_item_inline_var : module_item -> module_item := {
-    | AlwaysComb stmt => AlwaysComb (stmt_inline_var stmt)
-    }.
-
-  Equations
-    module_item_lst_inline_var : list module_item -> list module_item := {
+    apply_substitution_module_body : list module_item -> list module_item := {
     | [] => []
-    | (hd :: tl) => module_item_inline_var hd :: module_item_lst_inline_var tl
+    | ((AlwaysComb (BlockingAssign lhs rhs)) :: tl) =>
+       (AlwaysComb (BlockingAssign lhs (apply_substitution_expr rhs))) :: apply_substitution_module_body tl
     }.
-
-  Definition vmodule_inline_var (m : vmodule) : vmodule := {|
-    modName := modName m;
-    modVariableDecls := modVariableDecls m;
-    modBody := module_item_lst_inline_var (modBody m)
-  |}.
 End inline_one.
 
-Equations vmodule_inline_var_lst
-  : list substitution -> vmodule -> vmodule := {
-| [], m => m
-| (MkSubstitution var replacement :: tl), m =>
-  vmodule_inline_var var replacement (vmodule_inline_var_lst tl m)
-}.
+Lemma apply_substitution_module_body_length v r l :
+  List.length (apply_substitution_module_body v r l) = List.length l.
+Proof. funelim (apply_substitution_module_body v r l); crush. Qed.
 
-Equations module_item_collect_substitution (mi : module_item) : string + substitution := {
-| AlwaysComb (BlockingAssign (NamedExpression var) rhs) => inr (MkSubstitution var rhs)
-| AlwaysComb _ => inl "always_comb block with invalid structure in inlining stage"
-}.
-
-Equations module_item_lst_collect_substitutions (mis : list module_item) : string + list substitution := {
+Equations forward_assignments_body (mis : list module_item) : string + list module_item by wf (List.length mis) lt := {
 | [] => inr []
-| (hd :: tl) =>
-  let* sub := module_item_collect_substitution hd in
-  let* subs := module_item_lst_collect_substitutions tl in
-  inr (sub :: subs)
+| (AlwaysComb (BlockingAssign (NamedExpression var) rhs) :: tl) =>
+  let* tl' := forward_assignments_body (apply_substitution_module_body var rhs tl) in
+  inr (AlwaysComb (BlockingAssign (NamedExpression var) rhs) :: tl')
+| (_ :: _) => inl "always_comb block with invalid structure in inlining stage"
 }.
+Next Obligation. rewrite apply_substitution_module_body_length. lia. Qed.
+
+Definition forward_assignments (m : vmodule) : string + vmodule :=
+  assert_dec (List.NoDup (module_body_writes (modBody m))) "Duplicate write";;
+  assert_dec (module_items_sorted (module_inputs m) (modBody m)) "Module items unsorted" ;;
+  let* body := forward_assignments_body (modBody m) in
+  inr {|
+    modName := modName m;
+    modVariableDecls := modVariableDecls m;
+    modBody := body
+  |}.
 
 Equations target_pred : (variable -> bool) -> module_item -> bool := {
 | p, AlwaysComb (BlockingAssign (NamedExpression var) rhs) => p var
@@ -98,7 +80,7 @@ Equations target_pred : (variable -> bool) -> module_item -> bool := {
 
 (* TODO: Handle decls, and do in separate pass *)
 (* TODO: also: deshittify *)
-Definition vmodule_keep_only_outputs (m : vmodule) : vmodule := {|
+Definition vmodule_drop_internal (m : vmodule) : vmodule := {|
   modName := modName m;
   modVariableDecls := List.filter
    (fun d => match (varDeclPort d) with | Some _ => true | None => false end)
@@ -109,7 +91,3 @@ Definition vmodule_keep_only_outputs (m : vmodule) : vmodule := {|
       (module_outputs m)))
     (modBody m)
 |}.
-
-Definition forward_assignments (m : vmodule) : string + vmodule :=
-  let* substitutions := module_item_lst_collect_substitutions (modBody m) in
-  inr (vmodule_keep_only_outputs (vmodule_inline_var_lst substitutions m)).
